Foundation/Modal/Kripke/Hilbert/S4Point3.lean
@@ -6,19 +6,19 @@ namespace LO.Modal
 open Kripke
 open Geachean
 
-abbrev Kripke.connected_preorder : FrameClass := { F | Reflexive F ∧ Transitive F ∧ Connected F }
+abbrev Kripke.FrameClass.connected_preorder : FrameClass := { F | Reflexive F ∧ Transitive F ∧ Connected F }
 
 namespace Kripke.ReflexiveTransitiveConnectedFrameClass
 
-instance : FrameClass.DefinedBy Kripke.connected_preorder Hilbert.S4Point3.axioms := by
+instance : FrameClass.DefinedBy Kripke.FrameClass.connected_preorder Hilbert.S4Point3.axioms := by
   rw [
-    (show Kripke.connected_preorder = FrameClass.preorder ∩ FrameClass.connected by aesop),
+    (show Kripke.FrameClass.connected_preorder = FrameClass.preorder ∩ FrameClass.connected by aesop),
     (show Hilbert.S4Point3.axioms = Hilbert.S4.axioms ∪ {Axioms.Point3 (.atom 0) (.atom 1)} by aesop)
   ];
   exact FrameClass.definedBy_inter FrameClass.preorder (Hilbert.S4.axioms) FrameClass.connected {Axioms.Point3 (.atom 0) (.atom 1)};
 
 @[simp]
-protected lemma nonempty : Kripke.connected_preorder.Nonempty := by
+protected lemma nonempty : Kripke.FrameClass.connected_preorder.Nonempty := by
   use whitepoint.toFrame;
   simp [Reflexive, Transitive, Connected];
 
@@ -27,14 +27,14 @@ end Kripke.ReflexiveTransitiveConnectedFrameClass
 
 namespace Hilbert.S4Point3.Kripke
 
-instance sound : Sound (Hilbert.S4Point3) Kripke.connected_preorder := inferInstance
+instance sound : Sound (Hilbert.S4Point3) Kripke.FrameClass.connected_preorder := inferInstance
 
-instance consistent : Entailment.Consistent (Hilbert.S4Point3) := Hilbert.consistent_of_FrameClass Kripke.connected_preorder
+instance consistent : Entailment.Consistent (Hilbert.S4Point3) := Hilbert.consistent_of_FrameClass Kripke.FrameClass.connected_preorder
 
-instance canonical : Canonical (Hilbert.S4Point3) Kripke.connected_preorder :=
+instance canonical : Canonical (Hilbert.S4Point3) Kripke.FrameClass.connected_preorder :=
   ⟨⟨Canonical.reflexive, Canonical.transitive, Canonical.connected⟩⟩
 
-instance complete : Complete (Hilbert.S4Point3) Kripke.connected_preorder := inferInstance
+instance complete : Complete (Hilbert.S4Point3) Kripke.FrameClass.connected_preorder := inferInstance
 
 end Hilbert.S4Point3.Kripke
 
