Foundation/Modal/Logic/Sublogic/KTc.lean
@@ -9,12 +9,12 @@ open Kripke
 instance : ProperSublogic Logic.KTc Logic.Triv := ⟨by
   constructor;
   . exact Hilbert.weakerThan_of_dominate_axioms (by simp) |>.subset;
-  . suffices ∃ φ, Hilbert.Triv ⊢! φ ∧ ¬CoreflexiveFrameClass ⊧ φ by
+  . suffices ∃ φ, Hilbert.Triv ⊢! φ ∧ ¬FrameClass.corefl ⊧ φ by
       simpa [KTc.eq_CoreflexiveKripkeFrameClass_Logic];
     use (Axioms.T (.atom 0));
     constructor;
     . exact axiomT!;
-    . apply Formula.Kripke.ValidOnFrameClass.not_of_exists_model_world;
+    . apply Kripke.not_validOnFrameClass_of_exists_model_world;
       use ⟨⟨Fin 2, λ x y => False⟩, λ w _ => False⟩, 0;
       constructor;
       . simp [Coreflexive];
@@ -27,12 +27,12 @@ instance : ProperSublogic Logic.KTc Logic.Ver := ⟨by
     rintro φ hφ F F_iso;
     apply hφ;
     simp_all [Coreflexive, Isolated];
-  . suffices ∃ φ, Hilbert.Ver ⊢! φ ∧ ¬CoreflexiveFrameClass ⊧ φ by
+  . suffices ∃ φ, Hilbert.Ver ⊢! φ ∧ ¬FrameClass.corefl ⊧ φ by
       simpa [KTc.eq_CoreflexiveKripkeFrameClass_Logic];
     use (Axioms.Ver ⊥);
     constructor;
     . exact axiomVer!;
-    . apply Formula.Kripke.ValidOnFrameClass.not_of_exists_model_world;
+    . apply Kripke.not_validOnFrameClass_of_exists_model_world;
       let M : Model := ⟨⟨Fin 1, λ x y => True⟩, λ w _ => False⟩;
       use M, 0;
       constructor;
@@ -58,7 +58,7 @@ instance : ProperSublogic Logic.KB4 Logic.KTc := ⟨by
     use (Axioms.Tc (.atom 0));
     constructor;
     . exact axiomTc!;
-    . apply Formula.Kripke.ValidOnFrameClass.not_of_exists_model_world;
+    . apply Kripke.not_validOnFrameClass_of_exists_model_world;
       let M : Model := ⟨⟨Fin 2, λ x y => True⟩, λ w _ => w = 0⟩;
       use M, 0;
       constructor;
