Foundation/Modal/Logic/Sublogic/S5Grz.lean
@@ -9,11 +9,11 @@ open Kripke
 lemma S5_ssubset_S5Grz : Logic.S5 ⊂ Logic.S5Grz := by
   constructor;
   . exact Hilbert.weakerThan_of_dominate_axioms (by simp) |>.subset;
-  . suffices ∃ φ, Hilbert.S5Grz ⊢! φ ∧ ¬UniversalFrameClass ⊧ φ by simpa [S5.eq_UniversalKripkeFrameClass_Logic];
+  . suffices ∃ φ, Hilbert.S5Grz ⊢! φ ∧ ¬FrameClass.universal ⊧ φ by simpa [S5.eq_UniversalKripkeFrameClass_Logic];
     use Axioms.Grz (.atom 0)
     constructor;
     . exact axiomGrz!;
-    . apply Formula.Kripke.ValidOnFrameClass.not_of_exists_model_world;
+    . apply Kripke.not_validOnFrameClass_of_exists_model_world;
       use ⟨⟨Fin 2, λ x y => True⟩, λ w _ => w = 1⟩, 0;
       simp [Universal, Semantics.Realize, Satisfies];
 instance : ProperSublogic Logic.S5 Logic.S5Grz := ⟨S5_ssubset_S5Grz⟩
