Foundation/Modal/Logic/WellKnown.lean
@@ -37,7 +37,7 @@ protected abbrev Empty : Logic := ∅
 protected abbrev Univ : Logic := Set.univ
 
 protected abbrev K4 : Logic := Hilbert.K4.logic
-lemma K4.eq_TransitiveKripkeFrameClass_Logic : Logic.K4 = Kripke.FrameClass.transitive.logic
+lemma K4.eq_TransitiveKripkeFrameClass_Logic : Logic.K4 = Kripke.FrameClass.trans.logic
   := eq_Hilbert_Logic_KripkeFrameClass_Logic
 
 
@@ -57,52 +57,52 @@ lemma K45.eq_TransitiveEuclideanKripkeFrameClass_Logic : Logic.K45 = Kripke.Fram
 
 
 protected abbrev K5 : Logic := Hilbert.K5.logic
-lemma K5.eq_EuclideanKripkeFrameClass_Logic : Logic.K5 = Kripke.EuclideanFrameClass.logic
+lemma K5.eq_EuclideanKripkeFrameClass_Logic : Logic.K5 = Kripke.FrameClass.eucl.logic
   := eq_Hilbert_Logic_KripkeFrameClass_Logic
 
 
 protected abbrev KB : Logic := Hilbert.KB.logic
-lemma KB.eq_SymmetricKripkeFrameClass_Logic : Logic.KB = Kripke.SymmetricFrameClass.logic
+lemma KB.eq_SymmetricKripkeFrameClass_Logic : Logic.KB = Kripke.FrameClass.symm.logic
   := eq_Hilbert_Logic_KripkeFrameClass_Logic
 
 
 protected abbrev KB4 : Logic := Hilbert.KB4.logic
-lemma KB4.eq_ReflexiveTransitiveKripkeFrameClass_Logic : Logic.KB4 = Kripke.SymmetricTransitiveFrameClass.logic
+lemma KB4.eq_ReflexiveTransitiveKripkeFrameClass_Logic : Logic.KB4 = Kripke.FrameClass.symm_trans.logic
   := eq_Hilbert_Logic_KripkeFrameClass_Logic
 
 
 protected abbrev KB5 : Logic := Hilbert.KB5.logic
-lemma KB5.eq_ReflexiveEuclideanKripkeFrameClass_Logic : Logic.KB5 = Kripke.SymmetricEuclideanFrameClass.logic
+lemma KB5.eq_ReflexiveEuclideanKripkeFrameClass_Logic : Logic.KB5 = Kripke.FrameClass.symm_eucl.logic
   := eq_Hilbert_Logic_KripkeFrameClass_Logic
 
 
 protected abbrev KD : Logic := Hilbert.KD.logic
-lemma KD.eq_SerialKripkeFrameClass_Logic : Logic.KD = Kripke.SerialFrameClass.logic
+lemma KD.eq_SerialKripkeFrameClass_Logic : Logic.KD = Kripke.FrameClass.serial.logic
   := eq_Hilbert_Logic_KripkeFrameClass_Logic
 
 
 protected abbrev KD4 : Logic := Hilbert.KD4.logic
-lemma KD4.eq_SerialTransitiveKripkeFrameClass_Logic : Logic.KD4 = Kripke.SerialTransitiveFrameClass.logic
+lemma KD4.eq_SerialTransitiveKripkeFrameClass_Logic : Logic.KD4 = Kripke.FrameClass.serial_trans.logic
   := eq_Hilbert_Logic_KripkeFrameClass_Logic
 
 
 protected abbrev KD45 : Logic := Hilbert.KD45.logic
-lemma KD45.eq_SerialTransitiveEuclideanKripkeFrameClass_Logic : Logic.KD45 = Kripke.SerialTransitiveEuclideanFrameClass.logic
+lemma KD45.eq_SerialTransitiveEuclideanKripkeFrameClass_Logic : Logic.KD45 = Kripke.FrameClass.serial_trans_eucl.logic
   := eq_Hilbert_Logic_KripkeFrameClass_Logic
 
 
 protected abbrev KD5 : Logic := Hilbert.KD5.logic
-lemma KD5.eq_SerialEuclideanKripkeFrameClass_Logic : Logic.KD5 = Kripke.SerialEuclideanFrameClass.logic
+lemma KD5.eq_SerialEuclideanKripkeFrameClass_Logic : Logic.KD5 = Kripke.FrameClass.serial_eucl.logic
   := eq_Hilbert_Logic_KripkeFrameClass_Logic
 
 
 protected abbrev KDB : Logic := Hilbert.KDB.logic
-lemma KDB.eq_SerialSymmetricKripkeFrameClass_Logic : Logic.KDB = Kripke.SerialSymmetricFrameClass.logic
+lemma KDB.eq_SerialSymmetricKripkeFrameClass_Logic : Logic.KDB = Kripke.FrameClass.serial_symm.logic
   := eq_Hilbert_Logic_KripkeFrameClass_Logic
 
 
 protected abbrev KT : Logic := Hilbert.KT.logic
-lemma KT.eq_ReflexiveKripkeFrameClass_Logic : Logic.KT = Kripke.ReflexiveFrameClass.logic
+lemma KT.eq_ReflexiveKripkeFrameClass_Logic : Logic.KT = Kripke.FrameClass.refl.logic
   := eq_Hilbert_Logic_KripkeFrameClass_Logic
 
 
@@ -117,26 +117,26 @@ lemma S4.eq_ReflexiveTransitiveKripkeFrameClass_Logic : Logic.S4 = Kripke.FrameC
 
 
 protected abbrev S4Point2 : Logic := Hilbert.S4Point2.logic
-lemma S4Point2.eq_ReflexiveTransitiveConfluentKripkeFrameClass_Logic : Logic.S4Point2 = Kripke.FrameClass.partial_confluent.logic
+lemma S4Point2.eq_ReflexiveTransitiveConfluentKripkeFrameClass_Logic : Logic.S4Point2 = Kripke.FrameClass.confluent_preorder.logic
   := eq_Hilbert_Logic_KripkeFrameClass_Logic
 
 
 protected abbrev S4Point3 : Logic := Hilbert.S4Point3.logic
-lemma S4Point3.eq_ReflexiveTransitiveConnectedKripkeFrameClass_Logic : Logic.S4Point3 = Kripke.connected_preorder.logic
+lemma S4Point3.eq_ReflexiveTransitiveConnectedKripkeFrameClass_Logic : Logic.S4Point3 = Kripke.FrameClass.connected_preorder.logic
   := eq_Hilbert_Logic_KripkeFrameClass_Logic
 
+
 protected abbrev S5 : Logic := Hilbert.S5.logic
-lemma S5.eq_ReflexiveEuclideanKripkeFrameClass_Logic : Logic.S5 = Kripke.ReflexiveEuclideanFrameClass.logic
+lemma S5.eq_ReflexiveEuclideanKripkeFrameClass_Logic : Logic.S5 = Kripke.FrameClass.refl_eucl.logic
   := eq_Hilbert_Logic_KripkeFrameClass_Logic
-lemma S5.eq_UniversalKripkeFrameClass_Logic : Logic.S5 = Kripke.UniversalFrameClass.logic
+lemma S5.eq_UniversalKripkeFrameClass_Logic : Logic.S5 = Kripke.FrameClass.universal.logic
   := eq_Hilbert_Logic_KripkeFrameClass_Logic
 
 protected abbrev S5Grz : Logic := Hilbert.S5Grz.logic
 
 
 protected abbrev GL : Logic := Hilbert.GL.logic
-lemma GL.eq_TransitiveIrreflexiveFiniteKripkeFrameClass_Logic : Logic.GL = FrameClass.finite_transitive_irreflexive.logic
-  := eq_Hilbert_Logic_KripkeFiniteFrameClass_Logic
+lemma GL.eq_TransitiveIrreflexiveFiniteKripkeFrameClass_Logic : Logic.GL = Kripke.FiniteFrameClass.trans_irrefl.logic := eq_Hilbert_Logic_KripkeFiniteFrameClass_Logic
 instance : (Logic.GL).Unnecessitation := inferInstance
 
 
@@ -144,24 +144,21 @@ protected abbrev KH : Logic := Hilbert.KH.logic
 
 
 protected abbrev Grz : Logic := Hilbert.Grz.logic
-lemma Grz.eq_ReflexiveTransitiveAntiSymmetricFiniteKripkeFrameClass_Logic : Logic.Grz = Kripke.ReflexiveTransitiveAntiSymmetricFiniteFrameClass.logic
+lemma Grz.eq_ReflexiveTransitiveAntiSymmetricFiniteKripkeFrameClass_Logic : Logic.Grz = Kripke.FiniteFrameClass.strict_preorder.logic
   := eq_Hilbert_Logic_KripkeFiniteFrameClass_Logic
 
 
 protected abbrev Triv : Logic := Hilbert.Triv.logic
-lemma Triv.eq_EqualityKripkeFrameClass_Logic : Logic.Triv = Kripke.EqualityFrameClass.logic
-  := eq_Hilbert_Logic_KripkeFrameClass_Logic
+lemma Triv.eq_EqualityKripkeFrameClass_Logic : Logic.Triv = Kripke.FrameClass.equality.logic := eq_Hilbert_Logic_KripkeFrameClass_Logic
 
 
 protected abbrev Ver : Logic := Hilbert.Ver.logic
 instance : (Logic.Ver).Normal := Hilbert.normal
-lemma Ver.eq_IsolatedFrameClass_Logic : Logic.Ver = FrameClass.isolated.logic
-  := eq_Hilbert_Logic_KripkeFrameClass_Logic
+lemma Ver.eq_IsolatedFrameClass_Logic : Logic.Ver = Kripke.FrameClass.isolated.logic := eq_Hilbert_Logic_KripkeFrameClass_Logic
 
 
 protected abbrev KTc : Logic := Hilbert.KTc.logic
-lemma KTc.eq_CoreflexiveKripkeFrameClass_Logic : Logic.KTc = Kripke.CoreflexiveFrameClass.logic
-  := eq_Hilbert_Logic_KripkeFrameClass_Logic
+lemma KTc.eq_CoreflexiveKripkeFrameClass_Logic : Logic.KTc = Kripke.FrameClass.corefl.logic := eq_Hilbert_Logic_KripkeFrameClass_Logic
 
 end Logic
 
